\documentclass{article}
\usepackage{amsmath}
\begin{document}

$$
\vec v_1 =
\begin{bmatrix}
  x_1 \\
  y_1
\end{bmatrix}
=
\begin{bmatrix}
  x_0 + \Delta t \cdot (px_0 + qy_0) \\
  y_0 + \Delta t \cdot (rx_0 + sy_0)
\end{bmatrix}
=
\begin{bmatrix}
  (1 + \Delta t \cdot p)x_0 + \Delta t \cdot qy_0 \\
  \Delta t \cdot rx_0 + (1 + \Delta t \cdot s)y_0
\end{bmatrix}
=
\begin{bmatrix}
  (1 + \Delta t \cdot p) & \Delta t \cdot q \\
  \Delta t \cdot r & (1 + \Delta t \cdot s)
\end{bmatrix}
\begin{bmatrix}
  x_0 \\
  y_0
\end{bmatrix}
= 
B \cdot \vec v_0
$$

$$
A = 
\begin{bmatrix}
  -10^{-12} & 6 \cdot 10^7 \\
  10^{-12} & -6 \cdot 10^7
\end{bmatrix}
$$

$$\vec v(t) = 
\begin{bmatrix}
  N_1(t) \\
  N_2(t)
\end{bmatrix}
$$

$$
\vec v_0 =
\begin{bmatrix}
  1000 \\
  0
\end{bmatrix}
$$

$$
B = I + \Delta t \cdot A
= \begin{bmatrix}
  1 + \Delta t \cdot (-10^{-12}) & \Delta t \cdot 6 \cdot 10^7 \\
  \Delta t \cdot 10^{-12} & 1 + \Delta t \cdot (-6 \cdot 10^7)
\end{bmatrix}
$$


$$
\vec v_n = B^n \cdot \vec v_0
$$


\end{document}

